Made AppUnit in data complete

compiler/backend/semantics/bviSemScript.sml
@@ -195,10 +195,14 @@ End
 
 Definition AppUnit_def:
   AppUnit =
+      If (Op (BlockOp Equal)
+           [Op (IntOp (Const 0)) [];
+            Op (MemOp El) [Op (IntOp (Const 1)) []; Var 0]])
        (Call 0 NONE
              [Op (BlockOp (Cons 0)) []; Var 0;
               Op (MemOp El) [Op (IntOp (Const 0)) []; Var 0]]
              NONE)
+       (Call 0 (SOME num_stubs) [Op (BlockOp (Cons 0)) []; Var 0] NONE)
 End
 
 
